Evaluation/Example/plot2.py
@@ -30,7 +30,7 @@ for j in js:
         print("WARNING: {} was not processed entirely".format(j["fname"]))
 
 xs = [j["input_len"] for j in js]
-ys = [mean(j["times"]) for j in js]
+ys = [5*mean(j["times"]) for j in js]
 # e = [stdev(j["times"]) for j in js]
 e = [0 for j in js]
 
@@ -47,7 +47,43 @@ fig = plt.figure(figsize=(6,3))
 axis = fig.add_subplot(1, 1, 1)
 
 axis.plot(fxs,fys)
+axis.errorbar(xs, ys, yerr=e, fmt='go', ms=4)
+
+######
+
+input_dir = "results3"
+fs = listdir(input_dir)
+fs.sort(key = lambda x: int(x[:x.find(".")]))
+print(fs)
+fs = [input_dir+"/"+f for f in fs]
+# [:int(len(fs)/2)]
+cs = [fcontent(f) for f in fs]
+print(cs)
+js = [json.loads(c) for c in cs]
+
+for j in js:
+    if j["rest_len"] != 0:
+        print("WARNING: {} was not processed entirely".format(j["fname"]))
+
+xs = [j["input_len"] for j in js]
+ys = [mean(j["times"]) for j in js]
+# e = [stdev(j["times"]) for j in js]
+e = [0 for j in js]
+
+# for p in list(zip(xs,ys)):
+#     print("{} {}".format(p[0], p[1]))
+
+zs = np.polyfit(xs,ys,2)
+f = poly_eq(zs[::-1])
+# f = nlogn
+fxs = np.arange(0,max(xs),100)
+fys = [f(x) for x in fxs]
+
+
+axis.plot(fxs,fys)
 axis.errorbar(xs, ys, yerr=e, fmt='ro', ms=4)
+
+########
 
 axis.legend(["quadratic fit"])
 axis.set_xlabel("# Characters")
