Utils/ascii_order.v
@@ -2,7 +2,8 @@ Require Import List.
 Import ListNotations.
 Require Import Ascii.
 
-From Verbatim Require Import Utils.order.
+From Verbatim Require Import ltac.
+
 
 Definition ascii2list (a : ascii) : list bool :=
   match a with
@@ -10,25 +11,95 @@ Definition ascii2list (a : ascii) : list bool :=
     [b; b0; b1; b2; b3; b4; b5; b6]
   end.
 
-Definition bool_order (b1 b2 : bool) : order :=
+Lemma ascii2list_eq : forall x y,
+    x = y <-> ascii2list x = ascii2list y.
+Proof.
+  intros. split; intros.
+  - subst. auto.
+  - destruct x; destruct y. simpl in H.
+    injection H. intros; subst; auto.
+Qed.
+
+Definition bool_order (b1 b2 : bool) : comparison :=
   match b1, b2 with
-  | false, false => EQUAL
-  | false, true => LESSER
-  | true, false => GREATER
-  | true, true => EQUAL
+  | false, false => Eq
+  | false, true => Lt
+  | true, false => Gt
+  | true, true => Eq
   end.
+
+Lemma bool_order_eq : forall x y,
+    bool_order x y = Eq <-> x = y.
+Proof.
+  destruct x; destruct y; split; intros; try(discriminate); auto.
+Qed.
+
+Lemma bool_order_eq' : forall x,
+    bool_order x x = Eq.
+Proof.
+  intros. apply bool_order_eq. auto.
+Qed.
+
+Lemma bool_order_trans : forall c x y z,
+    bool_order x y = c -> bool_order y z = c -> bool_order x z = c.
+Proof.
+  intros. destruct x; destruct y; destruct z; auto; simpl in *; subst; discriminate.
+Qed.
   
-Fixpoint bool_list_order (bs bs' : list bool) : order :=
+Fixpoint bool_list_order (bs bs' : list bool) : comparison :=
   match bs, bs' with
-  | [], [] => EQUAL
-  | [], _ => LESSER
-  | _, [] => GREATER
+  | [], [] => Eq
+  | [], _ => Lt
+  | _, [] => Gt
   | h :: t, h' :: t' =>
     match bool_order h h' with
-    | EQUAL => bool_list_order t t'
+    | Eq => bool_list_order t t'
     | o => o
     end
   end.
 
-Definition ascii_order (a1 a2 : ascii) : order :=
+Lemma bool_list_order_eq : forall bs bs',
+    bool_list_order bs bs' = Eq <-> bs = bs'.
+Proof.
+  induction bs; destruct bs'; split; intros; try(discriminate); auto.
+  - destruct a; destruct b.
+    + simpl in H. apply IHbs in H. subst. auto.
+    + simpl in H. discriminate.
+    + simpl in H. discriminate.
+    + simpl in H. apply IHbs in H. subst. auto.
+  - injection H. intros. subst. simpl.
+    assert(bool_order b b = Eq).
+    { apply bool_order_eq. auto. }
+    rewrite H0. apply IHbs. auto.
+Qed.
+
+Lemma bool_list_order_trans : forall c x y z,
+    bool_list_order x y = c -> bool_list_order y z = c -> bool_list_order x z = c.
+Proof.
+  induction x; destruct y; destruct z; intros; auto;
+    try(simpl in *; rewrite <- H0 in *; discriminate).
+  simpl in *.
+  repeat dm;
+    try(rewrite bool_order_eq in *; subst; rewrite bool_order_eq' in *; discriminate);
+    try(apply bool_order_trans with (x:=a) in E; auto; rewrite E in E1; discriminate);
+    try(rewrite bool_order_eq in *; subst; rewrite E1 in *; discriminate).
+  - try(eapply IHx; eauto; reflexivity).
+  - rewrite bool_order_eq in *; subst. discriminate.
+  - rewrite bool_order_eq in *; subst. discriminate.
+Qed.
+
+Definition ascii_order (a1 a2 : ascii) : comparison :=
   bool_list_order (ascii2list a1) (ascii2list a2).
+
+Lemma ascii_order_eq : forall x y,
+    ascii_order x y = Eq <-> x = y.
+Proof.
+  intros. unfold ascii_order. rewrite ascii2list_eq. apply bool_list_order_eq.
+Qed.
+
+Lemma ascii_order_trans : forall c x y z,
+    ascii_order x y = c -> ascii_order y z = c -> ascii_order x z = c.
+Proof.
+  intros. unfold ascii_order in *. 
+  eapply bool_list_order_trans; eauto.
+Qed.
