Verbatim/memo/memo.v
@@ -2,6 +2,8 @@ Require Import List.
 Import ListNotations.
 
 From Verbatim Require Import state.
+From Verbatim Require Import lexer.correct.
+From Verbatim Require Import lexer.impl.
 
 Module Type MEMO (Import STT : state.T).
 
@@ -14,16 +16,43 @@ Module Type MEMO (Import STT : state.T).
   Parameter get_Memo : Memo -> State -> String -> option (option (String * String)).
 
   Parameter correct_Memo : forall M stt z o, get_Memo (set_Memo M stt z o) stt z = Some (o).
+  Parameter correct_Memo_moot : forall M stt stt' z z' o,
+      (stt <> stt' \/ z <> z')
+      -> 
+      get_Memo (set_Memo M stt' z' o) stt z = get_Memo M stt z.
   Parameter correct_emptyMemo : forall stt z, get_Memo emptyMemo stt z = None.
 
 End MEMO.
 
-(*Module MemoDefsFn (STT : state.T) (MEM : MEMO STT).*)
+Module MemoDefsFn (STT : state.T) (MEM : MEMO STT).
+
+  Import MEM.
+  Module Import NaiveLexer := lexer.impl.ImplFn STT.
+  Module Import NaiveLexerF := lexer.correct.CorrectFn STT.
+
+  
+  Definition lexy (M : Memo) : Prop :=
+    forall stt z o,
+      (get_Memo M stt z = Some o
+       -> max_pref_fn z stt = o)
+      (*/\ (max_pref_fn z stt = o
+         -> (get_Memo M stt z = Some o \/ get_Memo M stt z = None))*).
+
+  Definition lexy_list (Ms : list Memo) : Prop :=
+    forall M, In M Ms -> lexy M.
+
+
+End MemoDefsFn.
+
+Module Type DefsT (STT : state.T) (Ty : MEMO STT).
+  Include MemoDefsFn STT Ty.
+End DefsT.
 
 Module Type T.
   Declare Module STT : state.T.
-  Declare Module Ty : MEMO STT.
+  Declare Module MemTy : MEMO STT.
+  Declare Module Defs : DefsT STT MemTy.
   Export STT.
   Export STT.Ty.
-  Export Ty.
+  Export MemTy.
 End T.
