Verbatim/memo/concrete3.v
@@ -1,0 +1,47 @@
+Require Import List.
+Import ListNotations.
+
+Require Import FSets FSets.FMapAVL FSets.FMapFacts.
+
+From Verbatim Require Import state.
+From Verbatim Require Import memo.
+From Verbatim Require Import Orders.
+
+
+Module FMemo (STT : state.T) <: MEMO STT.
+
+  Import STT.Ty.
+  Import STT.Defs.
+  Import STT.R.Defs.
+
+  Module State_as_UOT <: UsualOrderedType := UOT_from_UCT State_as_UCT.
+  Module Suffix_as_UOT <: UsualOrderedType := List_as_UOT T_as_UOT.
+  Module pair_as_UOT <: UsualOrderedType := Pair_as_UOT State_as_UOT Suffix_as_UOT.
+
+  Module FM := FMapAVL.Make pair_as_UOT.
+  Module FMF := FMapFacts.Facts FM.
+
+  Definition Memo : Type := FM.t (option (String * String)).
+  Definition emptyMemo : Memo := FM.empty (option (String * String)).
+
+  Definition set_Memo (M : Memo) (stt : State) (sx : String) (o : (option (String * String))) :=
+    FM.add (stt, sx) o M.
+
+  Definition get_Memo (M : Memo) (stt : State) (sx : String) : option (option (String * String)) :=
+    FM.find (stt, sx) M.
+
+
+  Lemma correct_Memo : forall M stt z o, get_Memo (set_Memo M stt z o) stt z = Some (o).
+  Admitted.
+  
+  Lemma correct_Memo_moot : forall M stt stt' z z' o,
+      (stt <> stt' \/ z <> z')
+      -> 
+      get_Memo (set_Memo M stt' z' o) stt z = get_Memo M stt z.
+  Admitted.
+  
+  Lemma correct_emptyMemo : forall stt z, get_Memo emptyMemo stt z = None.
+  Admitted.
+  
+
+End FMemo.
