Verbatim/memo/correctness.v
@@ -1,0 +1,159 @@
+Require Import List.
+Import ListNotations.
+Require Import PeanoNat.
+Require Import Coq.omega.Omega.
+Require Import Coq.Numbers.NatInt.NZOrder.
+
+From Verbatim Require Import ltac.
+From Verbatim Require Import memo.
+From Verbatim Require Import memo.impl.
+
+Module CorrectFn (Import MEM : memo.T).
+
+  Import MEM.STT.Defs.
+  Import MEM.Defs.
+  Module Import IMPL := ImplFn MEM.
+  Import MEM.Defs.NaiveLexerF.
+  Import LEM.IMPL.Lex.
+  Import LEM.
+  Import IMPL.
+  Import MEMO.
+
+  Module Export CaseLemmas.
+
+    Lemma lex'_eq_body__M :
+      forall rules code Ms
+        (Ha : Acc lt (length code))
+        (Hlexy : lexy_list Ms)
+        (Hlen : length Ms = length rules),
+        (lex'__M Ms rules code Ha Hlexy Hlen =
+         (match max_of_prefs__M (max_prefs__M Ms code rules) as mpref'
+                return max_of_prefs__M (max_prefs__M Ms code rules) = mpref' -> _
+          with
+          | (Ms', _, None) => fun _ => (Ms', [], code) (* Code cannot be processed further *)
+          | (Ms', _, Some ([], _)) => fun _ => (Ms', [], code) (* Code cannot be processed further *)
+          | (Ms', label, Some (ph :: pt, suffix)) =>
+            fun Heq =>
+              match (lex'__M Ms' rules suffix
+                           (acc_recursive_call__M _ _ _ _ _ _ _ _ Ha Hlexy Hlen Heq)
+                           (lexy_recursive_call _ _ _ _ _ _ _ _ Hlexy Hlen Heq)
+                           (len_recursive_call _ _ _ _ _ _ _ _ Hlen Heq)
+                    )
+              with
+              | (Ms'', lexemes, rest) => (Ms'', ((label, ph :: pt) :: lexemes), rest)
+              end
+          end eq_refl)).
+    Proof.
+      intros rules code Ha Hlexy Hlen. unfold lex'.
+      destruct Ha; destruct Hlexy; auto.
+    Qed.
+
+    (*
+    Lemma lex'_cases_backward__M :
+      forall (Ms : list Memo)
+        (rules : list sRule)
+        (code : String)
+        (Ha : Acc lt (length code))
+        (Hlexy : lexy_list Ms)
+        (Hlen : length Ms = length rules)
+        (pr : list Memo * Label * option (Prefix * Suffix))
+        (res : list Memo * list Token * String)
+        (Heq : max_of_prefs__M (max_prefs__M Ms code rules) = pr),
+        match pr as mpref' return max_of_prefs__M (max_prefs__M Ms code rules) = mpref' -> _ with
+        | (Ms', _, None) => fun _ => ([], code) (* Code cannot be processed further *)
+        | (Ms', _, Some ([], _)) => fun _ => ([], code) (* Code cannot be processed further *)
+        | (Ms', label, Some (h :: t, suffix)) =>
+          fun Heq =>
+            match (lex'__M Ms' rules suffix
+                         (acc_recursive_call__M _ _ _ _ _ _ _ _ Ha Hlexy Hlen Heq)
+                         (lexy_recursive_call _ _ _ _ _ _ _ _ Hlexy Hlen Heq)
+                         (len_recursive_call _ _ _ _ _ _ _ _ Hlen Heq)
+                  )
+            with
+            | (Ms'', lexemes, rest) => (Ms'', ((label, h :: t) :: lexemes), rest)
+            end
+        end Heq = res.
+                        (*
+        -> match res with
+          | ([], code') =>
+            code' = code
+            /\ (snd pr = None
+               \/ exists suf, snd pr = Some ([], suf))
+          | ((label, prefix) :: lexemes, rest) =>
+            exists h t suffix (Heq' : max_of_prefs (max_prefs code rules) = (label, Some (h :: t, suffix))),
+            lex' rules suffix (acc_recursive_call _ _ _ _ _ _ Ha Heq') = (lexemes, rest)
+            /\ h :: t = prefix
+          end
+          end*).
+    Proof.
+      intros rules code Ha pr res Heq.
+      repeat dm; intros; subst; simpl in *; try congruence.
+      - split; inv H; eauto.
+      - inv H. exists s0. exists p1. exists s. exists Heq. split. apply E3. reflexivity.
+      - split; inv H; eauto.
+    Qed.*)
+
+    Lemma lex'_cases__M :
+      forall Ms rules code Ha Hlexy Hlen res,
+        lex'__M Ms rules code Ha Hlexy Hlen = res
+        -> match res with
+          | (_, [], code') =>
+            code' = code
+            /\ (snd (max_of_prefs__M (max_prefs__M Ms code rules)) = None
+               \/ exists suf, snd (max_of_prefs__M (max_prefs__M Ms code rules)) = Some ([], suf))
+          | (_, (label, prefix) :: lexemes, rest) =>
+            exists Ms'' Ms' h t suffix (Heq' : max_of_prefs__M (max_prefs__M Ms code rules)
+                                 = (Ms', label, Some (h :: t, suffix))),
+            lex'__M Ms' rules suffix
+                         (acc_recursive_call__M _ _ _ _ _ _ _ _ Ha Hlexy Hlen Heq')
+                         (lexy_recursive_call _ _ _ _ _ _ _ _ Hlexy Hlen Heq')
+                         (len_recursive_call _ _ _ _ _ _ _ _ Hlen Heq')
+            = (Ms'', lexemes, rest)
+            /\ h :: t = prefix
+          end.
+    (*
+    Proof.
+      intros rules code Ha res Heq; subst.
+      rewrite lex'_eq_body.
+      eapply lex'_cases_backward; eauto.
+    Qed.*)
+    Admitted.
+
+  End CaseLemmas.
+
+  Theorem lex'_memo_eq : forall rus code ts rest ts' rest' Ms,
+    lex' (map init_srule rus) code (lt_wf (length code)) = (ts, rest)
+    -> lex'__M (init_Memos (map init_srule rus)) (map init_srule rus) code
+         (lt_wf (length code)) (init_Memos_lexy (map init_srule rus))
+         (init_Memos_parallel (map init_srule rus)) = (Ms, ts', rest')
+    -> (ts, rest) = (ts', rest').
+  Proof.
+  Admitted.
+
+  Theorem lex_memo_eq : forall rus code,
+      lex__M rus code = lex rus code.
+  Proof.
+    intros. destruct (lex rus code) eqn:E.
+    unfold lex__M. unfold lex in E.
+    destruct (lex'__M (init_Memos (map Lex.init_srule rus)) (map Lex.init_srule rus) code
+                    (lt_wf (length code)) (init_Memos_lexy (map Lex.init_srule rus))
+                    (init_Memos_parallel (map Lex.init_srule rus))) eqn:E1.
+    destruct p.
+    eapply lex'_memo_eq in E1; eauto.
+  Qed.
+
+  Theorem lex_sound__M : forall ts code rest rus,
+      lex__M rus code = (ts, rest)
+      -> rules_is_function rus
+      -> tokenized rus code ts rest.
+  Proof.
+    intros. rewrite lex_memo_eq in *. apply lex_sound; auto.
+  Qed.
+
+  Theorem lex_complete__M : forall ts code rest rus,
+      tokenized rus code ts rest
+      -> rules_is_function rus
+      -> lex__M rus code = (ts, rest).
+  Proof.
+    intros. rewrite lex_memo_eq in *. apply lex_complete; auto.
+  Qed.
