Verbatim/memo/impl.v
@@ -1,0 +1,481 @@
+Require Import List.
+Import ListNotations.
+Require Import PeanoNat.
+Require Import Coq.omega.Omega.
+Require Import Coq.Numbers.NatInt.NZOrder.
+
+From Verbatim Require Import ltac.
+From Verbatim Require Import memo.
+From Verbatim Require Import lexer.impl.
+
+Module ImplFn (Import MEM : memo.T).
+
+  Module Import MEMO := MEM.MemTy.
+  Module Import Defs := MEM.Defs.
+  Import Defs.NaiveLexer.
+  Import MEM.STT.Defs.
+  Import MEM.STT.Ty.
+
+  Module Export Utils.
+
+    Fixpoint zip {A B : Type} (a: list A) (b: list B) : list (A * B) :=
+      match a, b with
+      | ha :: ta, hb :: tb => (ha,hb) :: (zip ta tb)
+      | _, _ => []
+      end.
+
+    Fixpoint unzip {A B : Type} (ab : list (A * B)) : (list A) * (list B) :=
+      match ab with
+      | [] => ([], [])
+      | (ha, hb) :: t =>
+        match unzip t with
+        | (ta, tb) => (ha :: ta, hb :: tb)
+        end
+      end.
+
+  End Utils.
+    
+  Module Export MPref.
+         
+    (** Single-rule Prefixer **)
+    Fixpoint max_pref_fn__M (M : Memo) (s : String) (state : State)
+    : Memo * option (String * String) :=
+      match s with
+      (* in a regex approach, accepting := nullable *)
+      | [] => if accepting state then (M, Some ([],[])) else (M, None)
+      | a :: s' =>
+        let
+          (* in a regex approach, transition := derivative *)
+          state' := transition a state in
+        let
+          lookup := get_Memo M state' s' in
+        let
+          mpxs :=
+          match lookup with
+          | None => max_pref_fn__M M s' state'
+          | Some o => (M, o)
+          end
+        in
+
+        match mpxs with
+        | (M', None) => if (accepting state') then (M' , Some ([a], s')) else
+                         if (accepting state) then (M', Some ([], s)) else
+                           ((set_Memo M' state s None), None)
+        | (M', Some (p, q)) => (M', Some (a :: p, q))
+        end
+      end.
+
+    (** Multi-rule Prefixer **)
+    Definition extract_fsm_for_max__M (code : String) (sru : Memo * (Label * State))
+      : Memo * (Label * option (Prefix * Suffix)) :=
+      match sru with
+        (M, (a, fsm)) =>
+        match max_pref_fn__M M code fsm with
+          (M', o) => (M', (a, o))
+        end
+      end.
+
+
+    Definition max_prefs__M (Ms : list Memo) (code : String) (erules : list (Label * State))
+      : (list Memo) * list (Label * option (Prefix * Suffix))
+      :=
+        let
+          zipped := zip Ms erules
+        in
+        let
+          mapped := map (extract_fsm_for_max__M code) zipped
+        in
+        unzip mapped.
+
+    Fixpoint max_of_prefs__M (mprefs : list Memo
+                                     * list (Label * (option (Prefix * Suffix))))
+      : list Memo * Label * option (Prefix * Suffix) :=
+      match mprefs with
+        (Ms, prefs) =>
+        match max_of_prefs prefs with
+          (l, o) => (Ms, l, o)
+        end
+      end.
+
+  End MPref.
+
+  Module Export TypeCheckLemmas.
+
+    Module Export MemoEq.
+
+      Lemma lexy_correct : forall M stt z o,
+        lexy M
+        -> get_Memo M stt z = Some (o)
+        -> max_pref_fn z stt = o.
+      Proof.
+        intros. unfold lexy in H. apply H in H0. auto.
+      Qed.
+
+      Theorem mpref_memo_eq_lexy_F : forall z stt o M M',
+          lexy M
+          -> max_pref_fn__M M z stt = (M', o)
+          -> max_pref_fn z stt = o.
+      Proof.
+        induction z; intros.
+        - simpl in *. repeat dm; repeat inj_all; auto.
+        - simpl in *.
+          repeat dm; repeat inj_all; auto;
+            try(eapply lexy_correct in H; eauto; rewrite E3 in H);
+            try(eapply IHz in H; eauto; rewrite E3 in H);
+            try(injection H; intros; subst; auto);
+            try(apply lexy_correct in E3; auto; rewrite E3 in E4; auto);
+            try(eapply IHz in H; eauto; rewrite E4 in H);
+            try(discriminate).
+      Qed.
+
+      Lemma cons_mprefs__M : forall m Ms z a rules m' Ms' p lst,
+          max_prefs__M (m :: Ms) z (a :: rules) = (m' :: Ms', p :: lst)
+          -> max_prefs__M [m] z [a] = ([m'], [p]) /\ max_prefs__M Ms z rules = (Ms', lst).
+      Proof.
+        intros. unfold max_prefs__M in *. simpl in *. repeat dm; repeat inj_all; subst. auto.
+      Qed.
+
+      Theorem mprefs_memo_F : forall z rules Ms Ms' lst,
+          lexy_list Ms
+          -> length Ms = length rules
+          -> max_prefs__M Ms z rules = (Ms', lst)
+          -> max_prefs z rules = lst.
+      Proof.
+        induction rules; intros.
+        - destruct Ms;
+            unfold max_prefs__M in H1; simpl in H1; repeat inj_all; subst; auto; discriminate.
+        - destruct Ms; try(discriminate).
+          assert(A0 : lexy_list Ms).
+          { unfold lexy_list in *. intros. apply H. simpl. right. auto. }
+          assert(A1 : length Ms = length rules).
+          { simpl in H0. inv H0. auto. }
+          destruct lst.
+          + unfold max_prefs__M in H1. simpl in H1. repeat dm. discriminate.
+          + destruct Ms'.
+            * unfold max_prefs__M in H1. simpl in H1. repeat dm. discriminate.
+            * simpl. unfold extract_fsm_for_max. dm. subst.
+              apply cons_mprefs__M in H1. eapply IHrules in A0; destruct H1; eauto.
+              unfold max_prefs__M in e. simpl in e. repeat dm. repeat inj_all; subst.
+              assert(A2 : lexy m).
+              { unfold lexy_list in *. apply H. simpl. left. auto. }
+              eapply mpref_memo_eq_lexy_F in A2; eauto. subst. auto.
+      Qed.
+
+    End MemoEq.
+
+    Module Export Accessible.
+      
+      Lemma acc_helper__M : forall Ms code rules Ms' label o,
+        lexy_list Ms
+        -> length Ms = length rules
+        -> max_of_prefs__M (max_prefs__M Ms code rules) = (Ms', label, o)
+        -> max_of_prefs (max_prefs code rules) = (label, o).
+      Proof.
+        intros. destruct (max_prefs code rules) eqn:E; destruct (max_prefs__M Ms code rules) eqn:E1.
+        - simpl in *. repeat dm; repeat inj_all; subst. eapply mprefs_memo_F in H; eauto.
+          + rewrite E in H. subst. simpl in E0. auto.
+        - simpl in *. repeat dm; repeat inj_all; subst. eapply mprefs_memo_F in H; eauto.
+          rewrite E in H. subst. simpl in E0. auto.
+      Qed.
+
+      Lemma acc_recursive_call__M :
+        forall code rules label s l suffix Ms Ms',
+          Acc lt (length code)
+          -> lexy_list Ms
+          -> length Ms = length rules
+          -> max_of_prefs__M (max_prefs__M Ms code rules) = (Ms', label, Some (s :: l, suffix))
+          -> Acc lt (length suffix).
+      Proof.
+        intros. eapply acc_helper__M in H0; eauto; eapply acc_recursive_call; eauto.
+      Defined.
+      
+
+    End Accessible.
+
+    Module Export Lengths.
+
+      Lemma memo_len_const : forall n Ms rules code Ms' l0,
+        n = length Ms'
+        -> length Ms = length rules
+        -> max_prefs__M Ms code rules = (Ms', l0)
+        -> length Ms' = length Ms.
+      Proof.
+        induction n; intros; destruct rules; destruct Ms; destruct Ms'; destruct l0;
+          try(simpl in *; auto; discriminate);
+          try(unfold max_prefs__M in *; simpl in *; repeat dm; repeat inj_all; subst; discriminate).
+        + simpl in *. injection H; intros; clear H. injection H0; intros; clear H0.
+          apply cons_mprefs__M in H1. destruct H1. eapply IHn in H2; eauto.
+      Qed.
+
+      Lemma labeled_len_const : forall n Ms rules code Ms' l0,
+          n = length Ms'
+          -> length Ms = length rules
+          -> max_prefs__M Ms code rules = (Ms', l0)
+          -> length Ms' = length l0.
+      Proof.
+        induction n; intros; destruct rules; destruct Ms; destruct Ms'; destruct l0;
+          try(simpl in *; auto; discriminate);
+          try(unfold max_prefs__M in *; simpl in *; repeat dm; repeat inj_all; subst; discriminate).
+        + simpl in *. injection H; intros; clear H. injection H0; intros; clear H0.
+          apply cons_mprefs__M in H1. destruct H1. eapply IHn in H2; eauto.
+      Qed.
+
+      Lemma all_lens_const' : forall n Ms rules code Ms' l0,
+          n = length Ms'
+          -> length Ms = length rules
+          -> max_prefs__M Ms code rules = (Ms', l0)
+          -> length Ms' = length Ms /\ length Ms' = length l0.
+      Proof.
+        intros. split.
+        - eapply memo_len_const; eauto.
+        - eapply labeled_len_const; eauto.
+      Qed.
+
+      Lemma all_lens_const : forall Ms rules code Ms' l0,
+          length Ms = length rules
+          -> max_prefs__M Ms code rules = (Ms', l0)
+          -> length Ms' = length Ms /\ length Ms' = length l0.
+      Proof.
+        intros. eapply all_lens_const'; eauto.
+      Qed.
+
+      Lemma len_recursive_call :
+        forall code rules label s l suffix Ms Ms',
+          length Ms = length rules
+          -> max_of_prefs__M (max_prefs__M Ms code rules) = (Ms', label, Some (s :: l, suffix))
+          -> length Ms' = length rules.
+      Proof.
+        intros. destruct (max_prefs__M Ms code rules) eqn:E.
+        assert(l0 = Ms').
+        {
+          simpl in H0. repeat dm. injection H0; auto.
+        }
+        subst. clear H0.
+        assert(L := all_lens_const Ms rules code Ms' l1 H E). destruct L. omega.
+      Qed.
+      
+    End Lengths.
+
+    Module Export LexyClosure.
+
+      Lemma nth_labels_match'' : forall m n rules Ms code Ms' l0 o ru label label',
+        m = length rules
+        -> length Ms = length rules
+        -> length rules = length l0
+        -> length Ms' = length Ms
+        -> n < length Ms'
+        -> max_prefs__M Ms code rules = (Ms', l0)
+        -> nth n l0 ([], None) = (label, o)
+        -> nth n rules ([], defState) = (label', ru)
+        -> label = label'.
+      Proof.
+        induction m; intros; destruct Ms; destruct rules; destruct Ms'; destruct l0; destruct n;
+          try(simpl in *; omega).
+        - apply cons_mprefs__M in H4. destruct H4. clear H7. simpl in *.
+          unfold max_prefs__M in H4. simpl in *. repeat dm; repeat inj_all. auto.
+        - simpl in *.
+          apply Nat.succ_inj in H.  apply Nat.succ_inj in H0.
+          apply Nat.succ_inj in H1. apply Nat.succ_inj in H2.
+          apply lt_S_n in H3.
+          apply cons_mprefs__M in H4. destruct H4.
+          eapply IHm; eauto.
+      Qed.
+
+      Lemma nth_labels_match' : forall m n rules Ms code Ms' l0 o ru label label',
+          m = length rules
+          -> length Ms = length rules
+          -> n < length Ms'
+          -> max_prefs__M Ms code rules = (Ms', l0)
+          -> nth n l0 ([], None) = (label, o)
+          -> nth n rules ([], defState) = (label', ru)
+          -> label = label'.
+      Proof.
+        intros.
+        assert(L := all_lens_const Ms rules code Ms' l0 H0 H2). destruct L.
+        eapply nth_labels_match''; eauto. omega.
+      Qed.
+
+      Lemma nth_labels_match : forall n rules Ms code Ms' l0 o ru label label',
+          max_prefs__M Ms code rules = (Ms', l0)
+          -> length Ms = length rules
+          -> n < length Ms'
+          -> nth n l0 ([], None) = (label, o)
+          -> nth n rules ([], defState) = (label', ru)
+          -> label = label'.
+      Proof.
+        intros. eapply nth_labels_match'; eauto.
+      Qed.
+
+      Lemma mprefs__M_associates :
+        forall n rules Ms Ms' code (l0 : list (Label * option (Prefix * Suffix))) M M' o label ru,
+          length Ms = length rules
+          -> max_prefs__M Ms code rules = (Ms', l0)
+          -> n < length Ms'
+          -> nth n Ms emptyMemo = M
+          -> nth n Ms' emptyMemo = M'
+          -> nth n l0 ([], None) = (label, o)
+          -> nth n rules ([], defState) = (label, ru)
+          -> max_pref_fn__M M code ru = (M', o).
+      Proof.
+        induction n; intros; destruct Ms; destruct Ms'; destruct l0; destruct rules;
+          try(simpl in *; omega);
+          try(rewrite nil_mprefs__M in *; repeat inj_all; discriminate);
+          try(simpl in *; repeat inj_all; unfold max_prefs__M in *; simpl in *;
+              repeat dm; repeat inj_all; discriminate).
+        + simpl in *. subst. unfold max_prefs__M in *. simpl in *.
+          repeat dm. repeat inj_all. auto.
+        + simpl in *. injection H; intros; clear H.
+          apply lt_S_n in H1. eapply IHn; eauto. eapply cons_mprefs__M; eauto.
+      Qed.
+
+      Lemma lexy_closure : 
+        forall code stt M o M',
+          lexy M
+          -> max_pref_fn__M M code stt = (M', o)
+          -> lexy M'.
+      Proof.
+        induction code; intros.
+        - simpl in H0. repeat dm; repeat inj_all; auto; discriminate.
+        - simpl in H0. destruct (get_Memo M (transition a stt) code) eqn:E.
+          + repeat dm; repeat inj_all; auto. clear IHcode.
+            unfold lexy. intros.
+            destruct (stt_eq_dec stt0 stt).
+            * destruct (String_dec z (a::code)).
+              -- subst. rewrite correct_Memo in H0. inv H0.
+                 unfold lexy in H. apply H in E. clear H.
+                 simpl. repeat dm; try(discriminate).
+              -- assert(L := correct_Memo_moot).
+                 specialize (L M stt0 stt z (a::code) None). rewrite L in H0; auto.
+            * assert(L := correct_Memo_moot).
+              specialize (L M stt0 stt z (a::code) None). rewrite L in H0; auto.
+          + repeat dm; repeat inj_all; auto; assert(E0' := E0); apply IHcode in E0; auto.
+            unfold lexy. intros.
+            destruct (stt_eq_dec stt0 stt).
+            * destruct (String_dec z (a::code)).
+              -- subst. rewrite correct_Memo in H0. inv H0.
+                 apply mpref_memo_eq_lexy_F in E0'; auto.
+                 simpl. repeat dm; try(discriminate).
+              -- assert(L := correct_Memo_moot).
+                 specialize (L m stt0 stt z (a::code) None). rewrite L in H0; auto.
+            * assert(L := correct_Memo_moot).
+              specialize (L m stt0 stt z (a::code) None). rewrite L in H0; auto.
+      Qed.
+
+      Lemma lexy_list_closure : 
+        forall code rules Ms l0 Ms',
+          lexy_list Ms
+          -> length Ms = length rules
+          -> max_prefs__M Ms code rules = (Ms', l0)
+          -> lexy_list Ms'.
+      Proof.
+        intros. unfold lexy_list in *. intros M' H2.
+        apply In_nth with (d := emptyMemo) in H2. destruct H2 as [n]. destruct H2.
+        assert(L := all_lens_const Ms rules code Ms' l0 H0 H1). destruct L.
+        assert(exists M, nth n Ms emptyMemo = M).
+        { eexists; eauto. }
+        destruct H6 as [M].
+        assert(exists label o, nth n l0 ([], None) = (label, o)).
+        { destruct (nth n l0 ([], None)). eexists; eauto. }
+        destruct H7 as [label]. destruct H7 as [o].
+        assert(exists label' ru, nth n rules ([], defState) = (label', ru)).
+        { destruct (nth n rules ([], defState)). eexists; eauto. }
+        destruct H8 as [label']. destruct H8 as [ru].
+        assert(label = label').
+        { eapply nth_labels_match; eauto. }
+        rewrite H9 in *. clear H9.
+        eapply mprefs__M_associates in H0; eauto.
+
+        assert(Hlen : length Ms = length Ms').
+        { omega. }
+        
+        rewrite <- Hlen in H2.
+        apply nth_In with (d:=emptyMemo) in H2. rewrite H6 in H2. apply H in H2.
+        eapply lexy_closure; eauto.
+      Qed.
+
+      Lemma lexy_recursive_call_gen :
+        forall code rules Ms label o Ms',
+          lexy_list Ms
+          -> length Ms = length rules
+          -> max_of_prefs__M (max_prefs__M Ms code rules) = (Ms', label, o)
+          -> lexy_list Ms'.
+      Proof.
+        intros. destruct (max_prefs__M Ms code rules) eqn:E.
+        assert(l = Ms').
+        {
+          simpl in H1. repeat dm. injection H1; auto.
+        }
+        subst. clear H1.
+        eapply lexy_list_closure in H; eauto.
+      Qed.
+
+      Lemma lexy_recursive_call :
+        forall code rules Ms label s l suffix Ms',
+          lexy_list Ms
+          -> length Ms = length rules
+          -> max_of_prefs__M (max_prefs__M Ms code rules) = (Ms', label, Some (s :: l, suffix))
+          -> lexy_list Ms'.
+        intros. eapply lexy_recursive_call_gen in H; eauto.
+      Qed.
+
+    End LexyClosure.
+    
+  End TypeCheckLemmas.
+
+  Module Export Lex.
+
+    Fixpoint lex'__M
+             (Ms : list Memo)
+             (rules : list (sRule))
+             (code : String)
+             (Ha : Acc lt (length code))
+             (Hlexy : lexy_list Ms)
+             (Hlen : length Ms = length rules)
+             {struct Ha} : (list Memo) * (list Token) * String :=
+      match max_of_prefs__M (max_prefs__M Ms code rules) as mpref'
+            return max_of_prefs__M (max_prefs__M Ms code rules) = mpref' -> _
+      with
+      | (Ms', _, None) => fun _ => (Ms', [], code) (* Code cannot be processed further *)
+      | (Ms', _, Some ([], _)) => fun _ => (Ms', [], code) (* Code cannot be processed further *)
+      | (Ms', label, Some (ph :: pt, suffix)) =>
+        fun Heq =>
+          match (lex'__M Ms' rules suffix
+                       (acc_recursive_call__M _ _ _ _ _ _ _ _ Ha Hlexy Hlen Heq)
+                       (lexy_recursive_call _ _ _ _ _ _ _ _ Hlexy Hlen Heq)
+                       (len_recursive_call _ _ _ _ _ _ _ _ Hlen Heq)
+                )
+          with
+          | (Ms'', lexemes, rest) => (Ms'', ((label, ph :: pt) :: lexemes), rest)
+          end
+      end eq_refl.
+
+    Definition init_srule (rule : Rule) : sRule :=
+      match rule with
+      | (label, re) => (label, init_state re)
+      end.
+
+    Definition init_Memos (srules : list sRule) : list Memo :=
+      (map (fun x => emptyMemo) srules).
+
+    Lemma init_Memos_lexy : forall srules,
+        lexy_list (init_Memos srules).
+    Admitted.
+
+    Lemma init_Memos_parallel : forall srules,
+        length (init_Memos srules) = length srules.
+    Admitted.
+
+    Definition lex__M (rules : list Rule) (code : String) : list Token * String :=
+      let
+        srules := map init_srule rules
+      in
+      match
+        lex'__M (init_Memos srules) srules code
+              (lt_wf _) (init_Memos_lexy _) (init_Memos_parallel _)
+       with
+       | (_, ts, rest) => (ts, rest)
+       end.
+
+  End Lex.
+
+End ImplFn.
